pcuic/theories/PCUICContexts.v
@@ -619,38 +619,3 @@ Proof.
   induction 1; simpl. constructor. rewrite fold_context_snoc0.
   now constructor.
 Qed.
-
-Lemma map_subst_closedn (s : list term) (k : nat) l :
-  forallb (closedn k) l -> map (subst s k) l = l.
-Proof.
-  induction l; simpl; auto.
-  move/andP=> [cla cll]. rewrite IHl //.
-  now rewrite subst_closedn.
-Qed.
-
-Lemma closedn_extended_subst_gen Γ k k' : 
-  closedn_ctx k Γ -> 
-  forallb (closedn (k' + k + context_assumptions Γ)) (extended_subst Γ k').
-Proof.
-  induction Γ as [|[? [] ?] ?] in k, k' |- *; simpl; auto;
-  rewrite ?closedn_ctx_cons;
-   move/andP => [clΓ /andP[clb clt]].
-  - rewrite IHΓ //.
-    epose proof (closedn_subst (extended_subst Γ k') (k' + k + context_assumptions Γ) 0).
-    autorewrite with len in H. rewrite andb_true_r.
-    eapply H; auto.
-    replace (k' + k + context_assumptions Γ + #|Γ|)
-    with (k + #|Γ| + (context_assumptions Γ + k')) by lia.
-    eapply closedn_lift. eapply clb.
-  - apply andb_and. split.
-    * apply Nat.ltb_lt; lia.
-    * specialize (IHΓ k (S k') clΓ).
-      red. rewrite -IHΓ. f_equal. f_equal. lia.
-Qed.
-
-Lemma closedn_extended_subst Γ : 
-  closed_ctx Γ -> 
-  forallb (closedn (context_assumptions Γ)) (extended_subst Γ 0).
-Proof.
-  intros clΓ. now apply (closedn_extended_subst_gen Γ 0 0).
-Qed.
